\chapter{Gravitational Waves}
\section{Linearized gravity}
Roughly speaking this is gravitational waves, while the macro area is \emph{linearized gravity} which is the study of GR where $g_{\mu \nu }$ can be decomposed in
\[
g_{\mu \nu } = \eta _{\mu \nu }+ h_{\mu \nu }, \left( |h_{\mu \nu }|<<1 \right)
\]
and $h_{\mu \nu }$ is a symmetric matrix.
That's nothing new, right? What we assumed back then was
\begin{itemize}
\item weak field
\item motion of slow test particle\footnote{A \emph{test particle} is and idealized concept to study the properties of spacetime and gravitational fields without significantly disturbing them. Specifically
	\begin{itemize}
	\item Infinitesimally small, point particle
	\item Negligible mass and energy, no contribute to curvature of spacetime.
	\item Moves along geodesics
	\item Used to explore effects of spacetime curvature.
	\end{itemize}
	}
\item static field.
\end{itemize}
We will give up on the last two assumptions for our derivation.\par
As just said, we  will start from
\begin{equation}
g_{\mu \nu } = \eta _{\mu \nu } + h_{\mu \nu } 
\end{equation}
we want to find the \emph{inverse metric} $g^{\mu \nu }$, we know
\[
g^{\mu \nu }g_{\nu \rho  } = \delta ^{\mu }_{\rho }
\]
let's express $g^{\mu \nu }$ like
\begin{equation}\label{eq:inversemetric}
g^{\mu \nu } = \eta ^{\mu \nu } + \Delta ^{\mu \nu }
\end{equation}
we will keep from now on only terms that are linear in $h_{\mu \nu }$, so $O\left( h \right)$ or that have the same order of $h_{\mu \nu }$.\par
\begin{align}
	g^{\mu \nu }g_{\nu \rho } &= \delta ^{\mu }_{\rho } \nonumber\\
	\left( \eta ^{\mu \nu } +\Delta ^{\mu \nu } \right)\left( \eta _{\nu \rho }+h_{\nu \rho } \right) &= \delta ^{\mu }_{\rho } \nonumber\\
	\delta ^{\mu }_{\rho } + \eta ^{\mu \nu }h_{\nu \rho } + \Delta ^{\mu \nu }\eta _{\nu \rho } + O\left( h^{2} \right) &= \delta ^{\mu }_{\rho } \nonumber\\
	\eta ^{\mu \nu }h_{\nu \rho } + \Delta ^{\mu \nu }\eta _{\nu \rho } & = 0 \nonumber\\
	\eta ^{\alpha \rho }\Delta ^{\mu \nu }\eta _{\nu \rho } & = - \eta ^{\mu \nu }h_{\nu \rho }\eta ^{\alpha \rho } \nonumber\\
	\delta ^{\alpha }_{\nu }\Delta ^{\mu \nu } &= - \eta ^{\mu \nu }\eta ^{\alpha \rho }h_{\nu \rho } \nonumber\\
	\Delta ^{\mu \alpha } &= -\eta ^{\mu \nu }\eta ^{\alpha \rho }h_{\nu \rho } \nonumber\\
	\Delta ^{\mu \nu } &= -\eta ^{\mu \alpha }\eta ^{\nu \beta }h_{\alpha \beta }
\end{align}
in the last step we changed indices to insert it on eq.\ref{eq:inversemetric}:
\begin{equation}
g^{\mu \nu } = \eta ^{\mu \nu } + \Delta^{\mu \nu } = \eta ^{\mu \nu }- \eta ^{\mu \alpha }\eta ^{\nu \beta }h_{\alpha \beta }
\end{equation}
The theory we are studying is of a dynamical symmetric tensor that propagates in flat spacetime, where the word \emph{propagates} gives us an hint about our goal. This is to take take \emph{h} and rewrite the Einstein Equation that is a equation of motion. \par
How does \emph{h} transform under LTs?
\begin{align}
	g_{\mu ^{\prime }\nu ^{\prime }} &= \Lambda ^{\mu }_{\mu ^{\prime }} \Lambda ^{\nu }_{\nu ^{\prime }}g_{\mu \nu } = \nonumber\\
	&= \Lambda ^{\mu }_{\mu ^{\prime }}\Lambda ^{\nu }_{\nu ^{\prime }}\left( \eta _{\mu \nu }+h_{\mu \nu } \right) = \nonumber\\
	&= \eta _{\mu ^{\prime }\nu ^{\prime }} + \Lambda ^{\mu }_{\mu ^{\prime }}\Lambda ^{\nu }_{\nu ^{\prime }}h_{\mu \nu } = \nonumber\\
	&= \eta _{\mu ^{\prime }\nu ^{\prime }}+h_{\mu ^{\prime }\nu ^{\prime }}
\end{align}
\paragraph{Christoffel symbol}
Now we can compute the Christoffel symbol
\begin{align}
	\Gamma ^{\rho }_{\mu \nu } &= \frac{1}{2} g^{\rho \sigma }\left[ \partial_{\mu }g_{\sigma \nu } + \partial_{\nu }g_{\sigma \mu } - \partial_{\sigma }g_{\mu \nu } \right] = \nonumber\\
	&= \frac{1}{2} \eta ^{\rho \sigma }\left[ \partial_{\mu }h_{\sigma \nu }+\partial_{\nu }h_{\sigma \mu } - \partial_{\sigma }h_{\mu \nu } \right]
\end{align}
we kept just $\eta $ outside the square brackets because the partial derivatives inside them are already $O\left( h \right)$, since derivative of $\eta $ is null.\par
\paragraph{Riemann tensor}
\begin{align}
	R^{\rho }_{\sigma \mu \nu } = \partial_{\mu }\Gamma ^{\rho }_{\sigma \nu } - \partial_{\nu }\Gamma ^{\rho }_{\sigma \mu } + \Gamma \Gamma -\Gamma \Gamma  = \nonumber\\
				    = \frac{1}{2} \partial_{\mu } \left[ \eta ^{\rho \alpha }\left( \partial_{\sigma} h_{\alpha \nu }+ \partial_{\nu }h_{\alpha \sigma }- \partial_{\alpha }h_{\sigma \nu } \right) \right] - \nonumber\\
				     \frac{1}{2}\partial_{\nu }\left[ \eta ^{\rho \alpha }\left( \partial_{\sigma }h_{\alpha \mu } +\partial_{\mu }h_{\sigma \alpha }- \partial_{\alpha }h_{\sigma \mu } \right) \right] \nonumber
\end{align}
terms that are $\Gamma \Gamma $ as you can see are not linear in $h$.\par
Now we will lower the upper index of the Riemann tensor since it is easier to manipulate.
\begin{gather}
	R_{\lambda \sigma \mu \nu } \simeq \eta _{\lambda \rho }R^{\rho }_{\sigma \mu \nu } = \nonumber \\
	 =  \eta _{\lambda \rho }\eta ^{\rho \alpha } \left( \partial_{\mu }\partial_{\sigma }h _{\alpha \nu } + \partial_{\mu }\partial_{\nu }h_{\alpha \sigma }-\partial_{\mu }\partial_{\alpha }h_{\sigma \nu } \right) - \nonumber\\
	  \frac{1}{2}\eta _{\lambda \rho }\eta ^{\rho \alpha }\left( \partial_{\nu }\partial_{\sigma }h_{\alpha \mu } + \partial_{\nu }\partial_{\mu }h_{\sigma \alpha }-\partial_{\nu }\partial_{\alpha }h_{\sigma \mu } \right) =  \nonumber\\
	  = \frac{1}{2} \delta ^{\alpha }_{\lambda }\left[ \left( \ldots  \right)\left( \ldots  \right) \right] = \nonumber\\
	  = \frac{1}{2} \left[ \left( \partial_{\mu }\partial_{\sigma }h_{\lambda \nu } +\partial_{\mu }\partial_{\nu }h_{\lambda \sigma }-\partial_{\nu }\partial_{\lambda }h_{\sigma \nu } \right) - \left( \partial_{\nu }\partial_{\sigma }h_{\lambda \mu }+ \partial_{\nu }\partial_{\mu }h_{\sigma \lambda } - \partial_{\nu }\partial_{\lambda }h_{\sigma \mu } \right) \right] \nonumber\\
	 \text{ {\small Partial derivatives commute, \emph{h} is symmetric }} \nonumber\\
	 = \frac{1}{2} \left[ \partial_{\mu }\partial_{\sigma }h_{\lambda \nu }-\partial_{\mu }\partial_{\lambda }h_{\sigma \nu } - \partial_{\nu }\partial_{\sigma }h_{\lambda \mu } + \partial_{\nu }\partial_{\lambda }h_{\sigma \mu } \right]
\end{gather}
\paragraph{Ricci tensor}

\begin{gather}
R^{\mu }_{\sigma \mu \nu } = \frac{1}{2}\left[ \partial^{\mu }\partial_{\sigma }h_{\mu \nu }- \partial^{\mu }\partial_{\mu }h_{\sigma \nu } - \partial_{\nu }\partial_{\sigma }h^{\mu }_{\mu }+ \partial_{\nu }\partial^{\mu }h_{\sigma \mu } \right] \nonumber\\
R_{\sigma \nu } = \frac{1}{2} \left( \partial^{\mu }\partial_{\sigma }h_{\mu \nu } + \partial^{\mu }\partial_{\nu  }h_{\mu \sigma }+ \partial_{\sigma }\partial_{\nu }h-\Box h_{\sigma \nu } \right)\label{eq:lingriccitns}
\end{gather}
with
\begin{gather*}
h \equiv \eta ^{\mu \nu }h_{\mu \nu }, \text{ the trace of \emph{h} } \\
\Box = \partial_{\mu }\partial^{\mu } = -\partial^{2}_{t} + \partial^{2}_{x}+\partial^{2}_{y}+\partial^{2}_{z}
\end{gather*}
\paragraph{Ricci scalar}
\begin{equation}
R = \eta ^{\sigma \nu }R_{\sigma \nu } = \frac{1}{2}\left( \partial^{\mu }\partial^{\sigma }h_{\mu \sigma }+ \partial^{\mu }\partial^{\sigma }h_{\sigma \mu }-\Box h -\Box h \right)= \partial^{\mu }\partial^{\sigma }h_{\mu \sigma }-\Box h
\end{equation}

\subsection{Gauge Invariant}
In the context of linearized gravity, gauge invariance refers to the freedom to make certain transformations to the metric perturbation $h_{\mu \nu }$ without changing the physical content of the theory. In the linearized regime, this invariance implies that $h_{\mu \nu }$ can be transformed under an infinitesimal coordinate change
\[
x^{\mu } \to x^{\mu }+ \xi^{\mu }  
\]
$\xi $ is dependent on coordinates, is not a constant, and is small.\par
Let's see how we write the metric tensor in new coordinate system.
\begin{align}
	g_{\mu ^{\prime }\nu ^{\prime }} &= \frac{\partial x^{\mu }}{\partial x^{\mu ^{\prime }}} \frac{\partial x^{\nu }}{\partial x^{\nu ^{\prime }}} \left( \eta _{\mu \nu } +h_{\mu \nu } \right) = \nonumber\\
					 &= \left( \delta ^{\mu }_{\mu ^{\prime }} + \partial_{\mu ^{\prime }}\xi ^{\mu } \right)\left( \partial^{\nu }_{\nu ^{\prime }}+\xi ^{\nu } \right)\left( \eta _{\mu \nu }+h_{\mu \nu } \right) = \nonumber\\
	&= \eta _{\mu ^{\prime }\nu ^{\prime }} + h_{\mu ^{\prime }\nu ^{\prime }} +\partial_{\mu ^{\prime }}\xi _{\nu ^{\prime }}+\partial_{\nu ^{\prime }}\xi _{\mu ^{\prime }}
\end{align}
where the last three terms are
\begin{equation}
\partial^{\mu }_{\mu ^{\prime }}\partial^{\nu }_{\nu ^{\prime }}h_{\mu \nu } \equiv   h_{\mu ^{\prime }\nu ^{\prime }} +\partial_{\mu ^{\prime }}\xi _{\nu ^{\prime }}+\partial_{\nu ^{\prime }}\xi _{\mu ^{\prime }}
\end{equation}
we did this infinitesimal change of coordinates and we found that the metric is minkowskian plus a correction.\par
We have
\[
\begin{rcases*}
h_{\mu \nu }\\
h_{\mu \nu }+ 2\partial_{(\mu  }\xi _{\nu )}
\end{rcases*}
\text{ that are equivalent }
\]
they both describe the same physical perturbation. Indeed \emph{gauge invariance} allows $h_{\mu \nu } $ to be shifted as
\[
h_{\mu \nu }\to h_{\mu \nu }+\partial_{\mu }\xi _{\nu }+\partial_{\nu }\xi _{\mu }
\]
Now we can compute the variation of the linearized Riemann tensor under this transformation
\begin{gather*}
	\delta R_{\lambda \sigma \mu \nu } = \frac{1}{2}\left[ \partial_{\mu }\partial_{\sigma }\delta h_{\nu \lambda } - \partial_{\mu }\partial_{\lambda }\delta h_{\sigma \nu } - \partial_{\nu }\partial_{\sigma }\delta h_{\lambda \mu } + \partial_{\nu }\partial_{\lambda }\delta h_{\sigma \mu } \right]\\
	= \frac{1}{2}[ \colorbox{yellow}{\underline{$ \partial_{\mu }\partial_{\sigma }$}$( \partial_{\nu }\xi _{\lambda }$}+ \text{ \underline{$\partial_{\lambda }\xi _{\nu }$}} ) \colorbox{pink}{\underline{$-  \partial_{\mu }\partial_{\lambda }$}}\text{\underline{$( \partial_{\sigma }\xi _{\nu }$}}+ \colorbox{pink}{$ \partial_{\nu }\xi _{\sigma }$}) + \\
	\colorbox{yellow}{$ - \partial_{\nu }\partial_{\sigma }$}\left( \partial_{\lambda }\xi _{\mu }+ \colorbox{yellow}{$ \partial_{\mu }\xi _{\lambda } $}\right) + \colorbox{pink}{$ \partial_{\nu }\partial_{\lambda }$}\left( \partial_{\sigma }\xi _{\mu }+ \colorbox{pink}{$ \partial_{\mu }\xi _{\sigma }$} \right) ] 
\end{gather*}
As you see by colors and underlining each term cancel with an opposite other. Since the variation of the Riemann tensor is null, this transformation leaves Riemann tensor, Ricci tensor and scalar unchanged.
























